

# Laplace Transform Sample Problem 1

This problem is question 1.1 from the Fall 2023 QE exam:

Using Laplace methods, solve the following differential equation.

$$y'''(t) + 2y''(t) + y'(t) = \delta(t) \quad (1)$$

$$y(0) = 0, \quad y'(0) = 0 \quad (2)$$

## 1 Take the Laplace transform of both sides

$$\mathcal{L}[y'''(t) + 2y''(t) + y'(t)] = \mathcal{L}[\delta(t)] \quad (3)$$

Using the linearity property of the Laplace transform, we can separate the left side.

$$\mathcal{L}[y'''(t)] + 2\mathcal{L}[y''(t)] + \mathcal{L}[y'(t)] = \mathcal{L}[\delta(t)] \quad (4)$$

Then we can apply the Laplace transform to each term.

$$\mathcal{L}[y'''(t)] = s^3Y(s) - s^2y(0) - sy'(0) - y''(0) = s^3Y(s) - y''(0) \quad (5)$$

$$\mathcal{L}[y''(t)] = s^2Y(s) - sy(0) - y'(0) = s^2Y(s) \quad (6)$$

$$\mathcal{L}[y'(t)] = sY(s) - y(0) = sY(s) \quad (7)$$

$$(8)$$

Now substituting these into the equation and cancelling out zeroes from initial conditions gives:

$$s^3Y(s) - y''(0) + 2s^2Y(s) + sY(s) = \mathcal{L}[\delta(t)] \quad (9)$$

The Laplace transform of the delta function is 1, so we have:

$$s^3Y(s) + 2s^2Y(s) + sY(s) - y''(0) = 1 \quad (10)$$

## 2 Solve for Y(s)

Factoring out  $Y(s)$  on the left side:

$$Y(s)(s^3 + 2s^2 + s) - y''(0) = 1 \quad (11)$$

Rearranging to solve for  $Y(s)$ :

$$Y(s) = \frac{1 + y''(0)}{s^3 + 2s^2 + s} \quad (12)$$

Here,  $y''(0) = 0$  since the jump in  $\delta$  happens at  $t = 0$  and the function is continuous. This leaves us with:

$$Y(s) = \frac{1}{s^3 + 2s^2 + s} \quad (13)$$

$$= \frac{1}{s(s^2 + 2s + 1)} \quad (14)$$

$$= \frac{1}{s(s+1)^2} \quad (15)$$

### 3 Partial fraction decomposition

We can decompose  $Y(s)$  into partial fractions:

$$Y(s) = \frac{A}{s} + \frac{B}{s+1} + \frac{C}{(s+1)^2} \quad (16)$$

Multiplying both sides by the denominator  $s(s+1)^2$  gives:

$$1 = A(s+1)^2 + Bs(s+1) + Cs \quad (17)$$

To start solving for the constants, we can choose  $s = 0$ :

$$1 = A(0+1)^2 + B(0)(0+1) + C(0) \quad (18)$$

$$A = 1 \quad (19)$$

Now, we can choose  $s = -1$ :

$$1 = A(-1+1)^2 + B(-1)(-1+1) + C(-1) \quad (20)$$

$$1 = 0 + 0 - C \quad (21)$$

$$C = -1 \quad (22)$$

Finally, choose  $s = 1$ :

$$1 = A(1+1)^2 + B(1)(1+1) + C(1) \quad (23)$$

$$1 = 4A + 2B + C \quad (24)$$

$$1 = 4(1) + 2B - 1 \quad (25)$$

$$1 = 3 + 2B \quad (26)$$

$$-2 = 2B \quad (27)$$

$$B = -1 \quad (28)$$

Thus, we have:

$$Y(s) = \frac{1}{s} - \frac{1}{s+1} - \frac{1}{(s+1)^2} \quad (29)$$

## 4 Take the inverse Laplace transform

Now we can take the inverse Laplace transform to find  $y(t)$ :

$$y(t) = \mathcal{L}^{-1} \left[ \frac{1}{s} \right] - \mathcal{L}^{-1} \left[ \frac{1}{s+1} \right] - \mathcal{L}^{-1} \left[ \frac{1}{(s+1)^2} \right] \quad (30)$$

Using known inverse Laplace transforms:

$$\mathcal{L}^{-1} \left[ \frac{1}{s} \right] = 1 \quad (31)$$

$$\mathcal{L}^{-1} \left[ \frac{1}{s+1} \right] = e^{-t} \quad (32)$$

$$\mathcal{L}^{-1} \left[ \frac{1}{(s+1)^2} \right] = te^{-t} \quad (33)$$

Substituting these back in gives:

$$y(t) = 1 - e^{-t} - te^{-t} \quad (34)$$

$$\boxed{y(t) = 1 - e^{-t}(1+t)} \quad (35)$$

Nice.